Alternative heap-sort approach, mostly verified
Switch out the standard heap-sort, in which the heap points in the opposite
direction, for a list-of-heaps sort in which power-of-two-minus-one sized heaps
point in the correct direction within the array. This has the advantage that an
already sorted array is confirmed sorted without moving anything and in linear
time. It also "agrees" with the functional model.

Problem though, the mapping of the multiple heaps into the array gets painful
to reason about. Saving before trying a different approach.

basis/pure/heap_sort_in_funScript.sml
@@ -6,6 +6,7 @@
 
   Could potentially move out of CakeML to HOL4 sorting theories.
 *)
+
 Theory heap_sort_in_fun
 Ancestors
    list rich_list sorting container bag
@@ -446,5 +447,546 @@ Theorem heap_sort_perm:
   PERM (heap_sort R xs) xs
 Proof
   simp [GSYM PERM_LIST_TO_BAG, heap_sort_contents]
+QED
+
+Datatype:
+  simple_tree = Empty_Tree | Node 'a simple_tree simple_tree
+End
+
+Definition tree_top_less_def:
+  tree_top_less R Empty_Tree y = T /\
+  tree_top_less R (Node x _ _) y = R x y
+End
+
+Definition heap_tree_inv_def:
+  (heap_tree_inv R n Empty_Tree = (n = 0)) /\
+  (heap_tree_inv R n (Node y l r) = (n > 0 /\
+    heap_tree_inv R (n - 1) l /\ tree_top_less R l y /\
+    heap_tree_inv R (n - 1) r /\ tree_top_less R r y
+  ))
+End
+
+Theorem heap_tree_inv_empty_eq_eq[local]:
+  heap_tree_inv R n t ==> ((t = Empty_Tree) = (n = 0))
+Proof
+  Cases_on `t` \\ simp [heap_tree_inv_def]
+QED
+
+Definition heaps_tree_inv_def:
+  heaps_tree_inv R xs = (EVERY (\(t, n). heap_tree_inv R n t /\ n > 0) xs /\
+    SORTED (\(t1, _) (t2, _). case t1 of Empty_Tree => F | Node x _ _ =>
+        (case t2 of Empty_Tree => F | Node y _ _ => R y x)) xs
+  )
+End
+
+Theorem heaps_tree_inv_rec_def:
+  (heaps_tree_inv R [] = T) /\
+  (heaps_tree_inv R (x :: xs) = (heap_tree_inv R (SND x) (FST x) /\ SND x > 0 /\
+    ((xs <> []) ==> tree_top_less R (FST (HD xs)) (case x of (Node y _ _, _) => y)) /\
+    heaps_tree_inv R xs))
+Proof
+  simp [heaps_tree_inv_def]
+  \\ Cases_on `x` \\ simp []
+  \\ Cases_on `xs` \\ simp []
+  \\ rpt (pairarg_tac \\ fs [])
+  \\ BasicProvers.EVERY_CASE_TAC \\ simp []
+  \\ simp [hd (CONJUNCTS heap_tree_inv_def)]
+  \\ simp [tree_top_less_def]
+  \\ EQ_TAC \\ rw [] \\ simp []
+QED
+
+Definition tree_to_bag_def:
+  tree_to_bag Empty_Tree = {||} /\
+  tree_to_bag (Node x l r) = BAG_INSERT x (BAG_UNION (tree_to_bag l) (tree_to_bag r))
+End
+
+(* Insert into a balanced heap/tree maintaining the invariant. *)
+Definition insert_tree_inv_def:
+  insert_tree_inv R Empty_Tree x = Empty_Tree /\
+  insert_tree_inv R (Node _ l r) x = (case l of Empty_Tree => Node x l r
+    | Node lx _ _ => (case r of Empty_Tree => Node x l r
+    | Node rx _ _ => if R lx x /\ R rx x then Node x l r
+    else if R lx rx then Node rx l (insert_tree_inv R r x)
+    else Node lx (insert_tree_inv R l x) r
+  ))
+End
+
+Theorem insert_tree_inv_size:
+  simple_tree_size (K 0) (insert_tree_inv R t x) =
+  simple_tree_size (K 0) t
+Proof
+  Induct_on `t`
+  \\ simp [insert_tree_inv_def]
+  \\ BasicProvers.EVERY_CASE_TAC \\ simp []
+QED
+
+(* Insert into a chain of heap/trees. *)
+Definition insert_trees_inv_def:
+  (insert_trees_inv R [] x = []) /\
+  (insert_trees_inv R ((t1, n1) :: ts) x = (case ts of
+    | [] => [(insert_tree_inv R t1 x, n1)]
+    | (t2, n2) :: tl_ts =>
+        (case t1 of Empty_Tree =>
+            (* won't happen, leave list the same *) ((t1, n1) :: ts)
+        | Node _ l r => (case t2 of Empty_Tree =>
+            (* won't happen, leave list the same *) ((t1, n1) :: ts)
+        | Node t2x _ _ => if ~ (R t2x x) /\
+            ~ (case l of Empty_Tree => F | Node lx _ _ => R t2x lx) /\
+            ~ (case r of Empty_Tree => F | Node rx _ _ => R t2x rx)
+        then (Node t2x l r, n1) :: insert_trees_inv R ts x
+        else (insert_tree_inv R t1 x, n1) :: ts
+  ))))
+End
+
+Theorem insert_trees_inv_size:
+  MAP (simple_tree_size (K 0) o FST) (insert_trees_inv R ts x) =
+  MAP (simple_tree_size (K 0) o FST) ts
+Proof
+  measureInduct_on `LENGTH ts`
+  \\ Cases_on `ts`
+  \\ simp [insert_trees_inv_def]
+  \\ Cases_on `h`
+  \\ simp [insert_trees_inv_def]
+  \\ BasicProvers.EVERY_CASE_TAC \\ simp []
+  \\ simp [insert_tree_inv_size]
+QED
+
+Theorem insert_trees_inv_length =
+  Q.AP_TERM `LENGTH` insert_trees_inv_size |> REWRITE_RULE [LENGTH_MAP]
+
+Definition add_trees_step1_def:
+  add_trees_step1 ts x = (case ts of
+    (t1, n1) :: (t2, n2) :: ts2 => if n1 = n2
+        then (Node x t2 t1, n1 + 1) :: ts2
+        else (Node x Empty_Tree Empty_Tree, 1) :: ts
+  | _ => (Node x Empty_Tree Empty_Tree, 1) :: ts
+  )
+End
+
+Definition add_trees_def:
+  add_trees R ts x = insert_trees_inv R (add_trees_step1 ts x) x
+End
+
+Definition build_trees_def:
+  build_trees R ts [] = ts /\
+  build_trees R ts (x :: xs) = build_trees R (add_trees R ts x) xs
+End
+
+Definition extend_trees_def:
+  extend_trees R ts t n = (case t of
+    Empty_Tree => ts
+  | Node x l r => (let ord = (case ts of ((Node y _ _, _) :: _) => R y x | _ => T)
+    in if ord then (t, n) :: ts
+        else insert_trees_inv R ((t, n) :: ts) x
+  ))
+End
+
+Theorem extend_trees_size:
+  SUM (MAP (\t_n. simple_tree_size (K 0) (FST t_n)) (extend_trees R ts t n)) =
+    simple_tree_size (K 0) t + SUM (MAP (\t_n. simple_tree_size (K 0) (FST t_n)) ts)
+Proof
+  simp [extend_trees_def]
+  \\ BasicProvers.EVERY_CASE_TAC \\ simp []
+  \\ simp [REWRITE_RULE [combinTheory.o_DEF] insert_trees_inv_size]
+QED
+
+Definition pull_trees_def:
+  pull_trees R [] acc = acc /\
+  pull_trees R ((Empty_Tree, _) :: ts) acc = acc /\
+  pull_trees R ((Node x l r, n) :: ts) acc =
+    let ts2 = extend_trees R ts l (n - 1);
+        ts3 = extend_trees R ts2 r (n - 1)
+    in pull_trees R ts3 (x :: acc)
+Termination
+  WF_REL_TAC `measure (\(R, ts, acc). SUM (MAP (simple_tree_size (K 0) o FST) ts))`
+  \\ rw []
+  \\ simp [extend_trees_size]
+End
+
+Definition another_heap_sort_def:
+  another_heap_sort R xs = pull_trees R (build_trees R [] xs) []
+End
+
+(* Invariant preservation. *)
+Theorem insert_tree_inv_less[local]:
+  (case t of Node _ l r => tree_top_less R l y /\ tree_top_less R r y | _ => T) ==>
+  R x y ==>
+  transitive R ==> total R ==>
+  tree_top_less R (insert_tree_inv R t x) y
+Proof
+  Cases_on `t` \\ simp [insert_tree_inv_def, tree_top_less_def]
+  \\ BasicProvers.EVERY_CASE_TAC \\ simp []
+  \\ simp [tree_top_less_def]
+QED
+
+Theorem insert_tree_inv:
+  heap_tree_inv R n t ==>
+  transitive R ==> total R ==>
+  heap_tree_inv R n (insert_tree_inv R t x)
+Proof
+  qid_spec_tac `n`
+  \\ Induct_on `t`
+  \\ rw [insert_tree_inv_def]
+  \\ BasicProvers.EVERY_CASE_TAC \\ simp []
+  \\ gs [heap_tree_inv_def, tree_top_less_def]
+  \\ irule_at Any insert_tree_inv_less
+  \\ simp []
+  \\ metis_tac [total_lemma, transitive_lemma]
+QED
+
+Theorem insert_tree_inv_greater[local]:
+  R x y \/ (case l of Node ly _ _ => R x ly | _ => F) \/
+      (case r of Node ry _ _ => R x ry | _ => F) ==>
+  transitive R ==> total R ==>
+  ((l = Empty_Tree) = (r = Empty_Tree)) ==>
+  R x (case insert_tree_inv R (Node x_old l r) y of
+    Empty_Tree => Anything | Node z _ _ => z)
+Proof
+  simp [insert_tree_inv_def]
+  \\ BasicProvers.EVERY_CASE_TAC \\ simp []
+  \\ simp [tree_top_less_def]
+  \\ metis_tac [transitive_lemma, total_lemma]
+QED
+
+Theorem insert_tree_inv_contents:
+  tree_to_bag (insert_tree_inv R t x) = (case t of Empty_Tree => {||}
+    | Node _ l r => tree_to_bag (Node x l r))
+Proof
+  Induct_on `t`
+  \\ simp [insert_tree_inv_def, tree_to_bag_def]
+  \\ BasicProvers.EVERY_CASE_TAC \\ simp []
+  \\ simp [tree_to_bag_def]
+  \\ simp [BAG_UNION_INSERT]
+  \\ simp [BAG_INSERT_commutes]
+QED
+
+Theorem tree_top_less_mono:
+  tree_top_less R t x ==> R x y ==>
+  transitive R ==>
+  tree_top_less R t y
+Proof
+  Cases_on `t`
+  \\ simp [tree_top_less_def]
+  \\ metis_tac [transitive_lemma]
+QED
+
+Theorem tree_top_less_neg[local]:
+  (~ (case t of Empty_Tree => F | Node y _ _ => R x y)) ==>
+  total R ==>
+  tree_top_less R t x
+Proof
+  BasicProvers.EVERY_CASE_TAC \\ simp [tree_top_less_def]
+  \\ metis_tac [total_lemma]
+QED
+
+Theorem heap_tree_inv_mono:
+  heap_tree_inv R n (Node x l r) ==>
+  R x y ==> transitive R ==>
+  heap_tree_inv R n (Node y l r)
+Proof
+  simp [heap_tree_inv_def]
+  \\ metis_tac [tree_top_less_mono]
+QED
+
+Theorem insert_trees_inv_less[local]:
+  (case ts of [] => F | (Empty_Tree, _) :: _ => F | ((Node _ l r, _) :: ts2) =>
+    tree_top_less R l y /\ tree_top_less R r y /\
+    (ts2 <> [] ==> FST (HD (ts2)) <> Empty_Tree /\
+        tree_top_less R (FST (HD ts2)) y)) ==>
+  R x y ==>
+  transitive R ==> total R ==>
+  tree_top_less R (FST (HD (insert_trees_inv R ts x))) y
+Proof
+  BasicProvers.EVERY_CASE_TAC \\ simp []
+  \\ simp [insert_trees_inv_def]
+  \\ BasicProvers.EVERY_CASE_TAC \\ simp []
+  \\ rw []
+  \\ fs [tree_top_less_def, insert_tree_inv_less]
+QED
+
+Theorem insert_trees_inv:
+  heaps_tree_inv R ts ==>
+  transitive R ==> total R ==>
+  heaps_tree_inv R (insert_trees_inv R ts x)
+Proof
+  Induct_on `ts`
+  \\ simp [insert_trees_inv_def, pairTheory.FORALL_PROD, heaps_tree_inv_rec_def]
+  \\ rpt gen_tac
+  \\ ntac 2 BasicProvers.TOP_CASE_TAC
+  \\ simp [insert_tree_inv, heaps_tree_inv_rec_def]
+  \\ ntac 2 BasicProvers.TOP_CASE_TAC
+  \\ simp [insert_tree_inv, heaps_tree_inv_rec_def]
+  \\ fs [hd (CONJUNCTS heap_tree_inv_def)]
+  \\ csimp []
+  \\ rw [heaps_tree_inv_rec_def]
+  \\ simp [insert_tree_inv]
+  >- (
+    fs [heap_tree_inv_def, tree_top_less_def]
+    \\ rpt (dxrule tree_top_less_neg)
+    \\ simp []
+  )
+  >- (
+    irule insert_trees_inv_less
+    \\ fs [heap_tree_inv_def, tree_top_less_def]
+    \\ fsrw_tac [SFY_ss] [total_lemma]
+    \\ rpt strip_tac
+    \\ Cases_on `t` \\ fs []
+    \\ fs [heaps_tree_inv_rec_def, heap_tree_inv_def]
+  )
+  >- (
+    simp [tree_top_less_def]
+    \\ irule insert_tree_inv_greater
+    \\ fs [heap_tree_inv_def]
+    \\ rpt (dxrule heap_tree_inv_empty_eq_eq)
+    \\ simp []
+  )
+QED
+
+Theorem insert_trees_inv_contents:
+  EVERY (\p. FST p <> Empty_Tree) ts ==>
+  (FOLDR BAG_UNION {||} (MAP (tree_to_bag o FST) (insert_trees_inv R ts x)) =
+    (case ts of [] => {||}
+      | (Node _ l r, _) :: ts => BAG_UNION (tree_to_bag (Node x l r))
+          (FOLDR BAG_UNION {||} (MAP (tree_to_bag o FST) ts)))
+  )
+Proof
+  Induct_on `ts`
+  \\ simp [pairTheory.FORALL_PROD, insert_trees_inv_def, tree_to_bag_def]
+  \\ rw []
+  \\ BasicProvers.EVERY_CASE_TAC \\ simp []
+  \\ fs [heaps_tree_inv_rec_def, heap_tree_inv_def]
+  \\ gs []
+  \\ simp [insert_tree_inv_contents, tree_to_bag_def]
+  \\ simp [BAG_UNION_INSERT]
+  \\ simp [BAG_INSERT_commutes]
+QED
+
+Theorem insert_trees_non_empty:
+  EVERY (\p. FST p <> Empty_Tree) ts ==>
+  EVERY (\p. FST p <> Empty_Tree) (insert_trees_inv R ts x)
+Proof
+  Induct_on `ts`
+  \\ simp [pairTheory.FORALL_PROD, insert_trees_inv_def]
+  \\ rw []
+  \\ BasicProvers.EVERY_CASE_TAC \\ simp []
+  \\ gs []
+  \\ rw [insert_tree_inv_def]
+QED
+
+Theorem build_trees_contents:
+  EVERY (\p. FST p <> Empty_Tree) ts ==>
+  FOLDR BAG_UNION {||} (MAP (tree_to_bag o FST) (build_trees R ts xs)) =
+  BAG_UNION (LIST_TO_BAG xs) (FOLDR BAG_UNION {||} (MAP (tree_to_bag o FST) ts)) /\
+  EVERY (\p. FST p <> Empty_Tree) (build_trees R ts xs)
+Proof
+  qid_spec_tac `ts`
+  \\ Induct_on `xs`
+  \\ rw [build_trees_def]
+  \\ simp [add_trees_def, add_trees_step1_def]
+  \\ BasicProvers.EVERY_CASE_TAC \\ simp []
+  \\ fs []
+  \\ simp [insert_trees_inv_contents, insert_trees_non_empty, tree_to_bag_def]
+  \\ simp [BAG_UNION_INSERT]
+  \\ simp [BAG_INSERT_commutes, ASSOC_BAG_UNION, COMM_BAG_UNION]
+QED
+
+Theorem insert_tree_inv_adj[local]:
+  insert_tree_inv R (Node x_dc l r) x =
+  insert_tree_inv R (Node y_dc l r) x
+Proof
+  simp [insert_tree_inv_def]
+QED
+
+Theorem insert_tree_adj_inv[local]:
+  heap_tree_inv R n (insert_tree_inv R (Node x l r) x)
+  ==>
+  heap_tree_inv R n (insert_tree_inv R (Node x_dc l r) x)
+Proof
+  simp [insert_tree_inv_def]
+QED
+
+Theorem insert_trees_adj_inv1[local]:
+  heaps_tree_inv R (insert_trees_inv R ((Node x_dc l r, n) :: ts) x) ==>
+  heaps_tree_inv R (insert_trees_inv R ((Node y_dc l r, n) :: ts) x)
+Proof
+  simp [insert_trees_inv_def]
+  \\ BasicProvers.EVERY_CASE_TAC \\ simp []
+  \\ simp [insert_tree_inv_def]
+  \\ csimp [heaps_tree_inv_rec_def, heap_tree_inv_def]
+QED
+
+Theorem insert_trees_adj_inv2[local]:
+  heaps_tree_inv R ts ==>
+  heap_tree_inv R n (Node x_dc l r) ==>
+  transitive R ==> total R ==> reflexive R ==>
+  heaps_tree_inv R (insert_trees_inv R ((Node x_dc l r, n) :: ts) x)
+Proof
+  Cases_on `heaps_tree_inv R ((Node x_dc l r, n) :: ts)`
+  \\ simp [insert_trees_inv]
+  \\ rw []
+  \\ irule insert_trees_adj_inv1
+  \\ qexists_tac `case HD ts of (Node x _ _, _) => x`
+  \\ irule insert_trees_inv
+  \\ fs [heaps_tree_inv_rec_def, heap_tree_inv_def]
+  \\ Cases_on `FST (HD ts)` \\ Cases_on `HD ts` \\ Cases_on `ts` \\ fs []
+  \\ fs [tree_top_less_def]
+  \\ simp [heaps_tree_inv_rec_def, heap_tree_inv_def, tree_top_less_def]
+  \\ fs [relationTheory.reflexive_def]
+  \\ rw []
+  \\ drule_then irule tree_top_less_mono
+  \\ simp []
+  \\ metis_tac [total_lemma]
+QED
+
+Theorem insert_trees_adj_inv3[local]:
+  heaps_tree_inv R ts ==>
+  heap_tree_inv R (n - 1) l ==>
+  heap_tree_inv R (n - 1) r ==>
+  n > 0 ==>
+  transitive R ==> total R ==> reflexive R ==>
+  heaps_tree_inv R (insert_trees_inv R ((Node x_dc l r, n) :: ts) x)
+Proof
+  Cases_on `heap_tree_inv R n (Node (case l of Node y _ _ => y) l r) \/
+      heap_tree_inv R n (Node (case r of Node y _ _ => y) l r)`
+  >- (
+    rw [] \\ fs []
+    \\ irule insert_trees_adj_inv1
+    \\ irule_at Any insert_trees_adj_inv2
+    \\ simp []
+    \\ first_x_assum (irule_at Any)
+  )
+  >- (
+    rw [] \\ fs []
+    \\ fs [heaps_tree_inv_rec_def, heap_tree_inv_def]
+    \\ BasicProvers.EVERY_CASE_TAC \\ fs [tree_top_less_def]
+    \\ gs [relationTheory.reflexive_def]
+    \\ irule insert_trees_adj_inv1
+    \\ irule_at Any insert_trees_adj_inv2
+    \\ simp [heap_tree_inv_def, relationTheory.reflexive_def, tree_top_less_def]
+    \\ metis_tac [total_lemma]
+  )
+QED
+
+Theorem build_trees_inv:
+  heaps_tree_inv R ts ==>
+  transitive R ==> total R ==> reflexive R ==>
+  heaps_tree_inv R (build_trees R ts xs)
+Proof
+  qid_spec_tac `ts`
+  \\ Induct_on `xs`
+  \\ rw [build_trees_def]
+  \\ simp [add_trees_def, add_trees_step1_def]
+  \\ BasicProvers.EVERY_CASE_TAC \\ simp []
+  \\ simp []
+  \\ first_x_assum irule
+  \\ simp []
+  \\ irule insert_trees_adj_inv3
+  \\ fs [heaps_tree_inv_rec_def, heap_tree_inv_def, tree_top_less_def]
+QED
+
+Theorem extend_trees_contents[local]:
+  EVERY (\p. FST p <> Empty_Tree) ts ==>
+  FOLDR BAG_UNION {||} (MAP (tree_to_bag o FST) (extend_trees R ts t n)) =
+  BAG_UNION (tree_to_bag t) (FOLDR BAG_UNION {||} (MAP (tree_to_bag o FST) ts))
+Proof
+  simp [extend_trees_def]
+  \\ BasicProvers.EVERY_CASE_TAC \\ simp []
+  \\ simp [tree_to_bag_def]
+  \\ simp [insert_trees_inv_contents, insert_trees_non_empty, tree_to_bag_def]
+QED
+
+Theorem extend_trees_not_empty[local]:
+  EVERY (\p. FST p <> Empty_Tree) ts ==>
+  EVERY (\p. FST p <> Empty_Tree) (extend_trees R ts t n)
+Proof
+  simp [extend_trees_def]
+  \\ BasicProvers.EVERY_CASE_TAC \\ simp []
+  \\ simp [insert_trees_non_empty]
+QED
+
+Theorem extend_trees_inv[local]:
+  (t <> Empty_Tree ==> heap_tree_inv R n t) ==>
+  heaps_tree_inv R ts ==>
+  total R /\ transitive R /\ reflexive R ==>
+  heaps_tree_inv R (extend_trees R ts t n)
+Proof
+  simp [extend_trees_def]
+  \\ BasicProvers.EVERY_CASE_TAC \\ simp []
+  \\ csimp [heaps_tree_inv_rec_def, heap_tree_inv_def, tree_top_less_def]
+  \\ rw []
+  \\ irule insert_trees_adj_inv3
+  \\ fs [heaps_tree_inv_rec_def, heap_tree_inv_def]
+QED
+
+Theorem extend_trees_less[local]:
+  (ts <> [] ==> tree_top_less R (FST (HD ts)) x) ==>
+  tree_top_less R t x ==>
+  total R ==> transitive R ==>
+  (extend_trees R ts t n <> []) ==>
+  heaps_tree_inv R ts ==>
+  heap_tree_inv R n t ==>
+  tree_top_less R (FST (HD (extend_trees R ts t n))) x
+Proof
+  simp [extend_trees_def]
+  \\ BasicProvers.EVERY_CASE_TAC \\ simp []
+  \\ rw []
+  \\ irule insert_trees_inv_less
+  \\ fs [tree_top_less_def]
+  \\ fs [heaps_tree_inv_rec_def, heap_tree_inv_def]
+  \\ fsrw_tac [SFY_ss] [tree_top_less_mono]
+  \\ CCONTR_TAC
+  \\ Cases_on `ts`
+  \\ gs [heaps_tree_inv_rec_def, heap_tree_inv_def]
+QED
+
+Theorem pull_trees_contents:
+  ! R ts acc. EVERY (\p. FST p <> Empty_Tree) ts ==>
+  LIST_TO_BAG (pull_trees R ts acc) =
+  BAG_UNION (FOLDR BAG_UNION {||} (MAP (tree_to_bag o FST) ts)) (LIST_TO_BAG acc)
+Proof
+  recInduct pull_trees_ind
+  \\ rw []
+  \\ simp [pull_trees_def, tree_to_bag_def]
+  \\ simp [extend_trees_contents, extend_trees_not_empty]
+  \\ simp [BAG_UNION_INSERT]
+  \\ simp [BAG_INSERT_commutes, ASSOC_BAG_UNION, COMM_BAG_UNION]
+QED
+
+Theorem pull_trees_sorted:
+  ! R ts acc. heaps_tree_inv R ts ==>
+  transitive R ==> total R ==> reflexive R ==>
+  SORTED R acc ==>
+  ((ts <> []) ==> (acc <> []) ==> tree_top_less R (FST (HD ts)) (HD acc)) ==>
+  SORTED R (pull_trees R ts acc)
+Proof
+  recInduct pull_trees_ind
+  \\ rw [] \\ fs []
+  \\ simp [pull_trees_def]
+  \\ fs [heaps_tree_inv_rec_def, heap_tree_inv_def, tree_top_less_def]
+  \\ gs []
+  \\ first_x_assum irule
+  \\ simp [extend_trees_inv]
+  \\ rw []
+  \\ simp [extend_trees_less, extend_trees_inv]
+  \\ Cases_on `acc`
+  \\ fs []
+QED
+
+Theorem another_heap_sort_sorted:
+  reflexive R ==> transitive R ==> total R ==>
+  SORTED R (another_heap_sort R xs)
+Proof
+  rw [another_heap_sort_def]
+  \\ irule pull_trees_sorted
+  \\ simp []
+  \\ irule build_trees_inv
+  \\ simp [heaps_tree_inv_def]
+QED
+
+Theorem another_heap_sort_contents:
+  LIST_TO_BAG (another_heap_sort R xs) = LIST_TO_BAG xs
+Proof
+  rw [another_heap_sort_def]
+  \\ simp [pull_trees_contents, build_trees_contents]
 QED
 
